src/util/MonadTests.v
@@ -1,0 +1,232 @@
+Require Import Coq.Lists.List. Import ListNotations.
+Require Import Coq.Arith.PeanoNat.
+
+
+Class Monad(M: Type -> Type) := mkMonad {
+  Bind: forall {A B}, M A -> (A -> M B) -> M B;
+  Return: forall {A}, A -> M A;
+}.
+
+Notation "x <- m1 ; m2" := (Bind m1 (fun x => m2))
+  (right associativity, at level 60) : monad_scope.
+Notation "m1 ;; m2" := (Bind m1 (fun _ => m2))
+  (right associativity, at level 60) : monad_scope.
+
+Open Scope monad_scope.
+
+
+Definition Id: Type -> Type := id.
+
+Instance Id_monad: Monad Id := {|
+  Bind{A B}(m: A)(f: A -> B) := f m;
+  Return{A}(a: A) := a;
+|}.
+
+
+Record optionT(M: Type -> Type)(A: Type): Type := mkOptionT {
+  runOptionT: M (option A)
+}.
+Arguments mkOptionT {M} {A} (_).
+Arguments runOptionT {M} {A} (_).
+
+Instance OptionT_Monad(M: Type -> Type){MM: Monad M}: Monad (optionT M) := {|
+  Bind{A}{B}(m: optionT M A)(f: A -> optionT M B) :=
+    mkOptionT (Bind (runOptionT m) (fun (o: option A) =>
+                                      match o with
+                                      | Some a => runOptionT (f a)
+                                      | None => Return None
+                                      end));
+  Return{A}(a: A) := mkOptionT (Return (Some a));
+|}.
+
+Definition lift_into_optionT{M: Type -> Type}{MM: Monad M}{A: Type}(m: M A): optionT M A :=
+  mkOptionT (Bind m (fun a => Return (Some a))).
+
+Definition fail{A: Type}{M: Type -> Type}{MM: Monad M}: optionT M A :=
+  mkOptionT (Return None).
+
+
+Definition State(S A: Type) := S -> (A * S).
+
+Record StateT(S: Type)(M: Type -> Type)(A: Type): Type := mkStateT {
+  runStateT: S -> M (A * S)%type
+}.
+Arguments mkStateT {S} {M} {A} (_).
+Arguments runStateT {S} {M} {A} (_).
+
+Instance StateT_Monad(M: Type -> Type){MM: Monad M}(S: Type): Monad (StateT S M) := {|
+  Bind{A B: Type}(m: StateT S M A)(f: A -> StateT S M B) :=
+    mkStateT (fun (s: S) => Bind ((runStateT m) s) (fun '(a, s) => runStateT (f a) s));
+  Return{A: Type}(a: A) :=
+    mkStateT (fun (s: S) => Return (a, s));
+|}.
+
+Definition lift_into_StateT{S: Type}{M: Type -> Type}{MM: Monad M}{A: Type}(m: M A): StateT S M A :=
+  mkStateT (fun s => Bind m (fun a => Return (a, s))).
+
+Definition get{S: Type}{M: Type -> Type}{MM: Monad M}: StateT S M S :=
+  mkStateT (fun (s: S) => Return (s, s)).
+
+Definition put{S: Type}{M: Type -> Type}{MM: Monad M}(s: S): StateT S M unit :=
+  mkStateT (fun _ => Return (tt, s)).
+
+
+Record listT(M: Type -> Type)(A: Type): Type := mkListT {
+  runListT: M (list A)
+}.
+Arguments mkListT {M} {A} (_).
+Arguments runListT {M} {A} (_).
+
+Instance listT_Monad(M: Type -> Type){MM: Monad M}: Monad (listT M) := {|
+  Bind{A B: Type}(m: listT M A)(f: A -> listT M B) :=
+    mkListT (la <- runListT m;
+             List.fold_left
+               (fun res a =>
+                  res' <- res;
+                  a' <- runListT (f a);
+                  Return (res' ++ a'))
+               la
+               (Return (@nil B)));
+  Return{A: Type}(a: A) :=
+    mkListT (Return (cons a nil));
+|}.
+
+
+Definition lift_into_listT{M: Type -> Type}{MM: Monad M}{A: Type}(m: M A): listT M A :=
+  mkListT (Bind m (fun a => (Return (cons a nil)))).
+
+Definition pick{A: Type}{M: Type -> Type}{MM: Monad M}(options: list A): listT M A :=
+  mkListT (Return options).
+
+Definition comp1: listT Id (nat * bool) :=
+  x1 <- pick [3; 4];
+  x2 <- pick [true; false];
+  Return (x1, x2).
+
+Compute (runListT comp1).
+
+Definition comp2: (listT (optionT Id)) nat :=
+  b <- pick [true; false];
+  if (b: bool) then
+    pick [3; 4]
+  else
+    lift_into_listT fail.
+
+Compute (runOptionT (runListT comp2)).
+
+Definition comp3: (optionT (listT Id)) nat :=
+  b <- lift_into_optionT (pick [true; false]);
+  if (b: bool) then
+    lift_into_optionT (pick [3; 4])
+  else
+    fail.
+
+Compute (runListT (runOptionT comp3)).
+
+Definition comp4: StateT nat Id unit :=
+  x <- get;
+  put (x + 1).
+
+Compute (runStateT comp4 4).
+
+
+Definition comp5: StateT nat (listT Id) unit :=
+  x <- get;
+  y <- lift_into_StateT (pick [2; 3]);
+  put (x + y).
+
+Compute (runListT (runStateT comp5 4)).
+
+Compute (seq 0 4).
+
+Definition comp6: StateT nat (listT Id) unit :=
+  x <- get;
+  y <- lift_into_StateT (pick (seq 0 x));
+  put y.
+
+Compute (runListT (runStateT comp6 4)).
+
+
+Definition comp7: StateT nat (listT Id) unit :=
+  x <- get;
+  y <- lift_into_StateT (pick (seq 0 x));
+  if Nat.eq_dec y 2 then
+    put 22
+  else
+    put 11.
+
+
+Definition comp8: (listT (StateT nat Id) nat) :=
+  x <- lift_into_listT get;
+  y <- pick (seq 0 x);
+  lift_into_listT (put y);;
+  lift_into_listT get.
+
+Compute (runStateT (runListT comp8) 4).
+
+
+Definition comp9: (listT (StateT nat Id) nat) :=
+  x <- lift_into_listT get;
+  y <- pick (seq 0 x);
+  lift_into_listT (put y);;
+  (if Nat.eq_dec y 2 then
+    (c <- lift_into_listT get;
+     lift_into_listT (put (c * 3)))
+  else
+    (c <- lift_into_listT get;
+     lift_into_listT (put (c * 5))));;
+  lift_into_listT get.
+
+Compute (runStateT (runListT comp9) 4).
+
+Record Regs := mkRegs {
+  reg1: nat;
+  reg2: nat;
+  reg3: nat;
+}.
+
+Notation "<< x1 , x2 , x3 >>" := (mkRegs x1 x2 x3) (format "<< x1 , x2 , x3 >>").
+
+Inductive Reg := r1 | r2 | r3.
+
+Definition getReg(r: Reg): StateT Regs Id nat :=
+  s <- get;
+  Return (match r with
+          | r1 => s.(reg1)
+          | r2 => s.(reg2)
+          | r3 => s.(reg3)
+          end).
+
+Definition setReg(r: Reg)(v: nat): StateT Regs Id unit :=
+  s <- get;
+  put (match r with
+       | r1 => mkRegs v        s.(reg2) s.(reg3)
+       | r2 => mkRegs s.(reg1) v        s.(reg3)
+       | r3 => mkRegs s.(reg1) s.(reg2) v
+       end).
+
+Definition assign(ra rb: Reg): StateT Regs Id unit :=
+  x <- getReg rb;
+  setReg ra x.
+
+Definition swap12: StateT Regs Id unit :=
+  assign r3 r1;;
+  assign r1 r2;;
+  assign r2 r3.
+
+Compute (runStateT swap12 (mkRegs 10 20 30)).
+
+Definition test1: listT (StateT Regs Id) Regs :=
+  x <- lift_into_listT (getReg r1);
+  y <- pick (seq 0 x);
+  lift_into_listT (setReg r1 y);;
+  lift_into_listT get.
+
+(* returns a list of all final states as "answer"
+   and one implementation-chosen final state as "state" *)
+Compute (runStateT (runListT test1) (mkRegs 3 20 30)).
+
+Definition test2: listT (StateT Regs Id) Regs :=
+  lift_into_listT swap12;; test1.
+
+Compute (runStateT (runListT test2) (mkRegs 11 4 33)).
